\documentclass{article}

\title{NE 400 Homework 3}
\author{Daniel Nevius}
\date{February 20th, 2023}

\begin{document}

\maketitle

\section{}


Cycle Efficiency:
\begin{equation}
\eta_{a} = \frac{\dot{W}_{htp    } / \dot{m}_{1} + \dot{W}_{ltp    } / \dot{m}_{1} + \dot{W}_{cp     } / \dot{m}_{1} + \dot{W}_{cbp    } / \dot{m}_{1} + \dot{W}_{fp1    } / \dot{m}_{1} + \dot{W}_{fp2    } / \dot{m}_{1}}{\dot{Q}_{SG1    } / \dot{m}_{1} + \dot{Q}_{SG2    } / \dot{m}_{1}}
\end{equation}

\begin{equation}
\eta_{t} =    0.950
\end{equation}

\begin{equation}
\eta_{p} =    0.800
\end{equation}

\begin{equation}
x_{ 2} =   95.000\%
\end{equation}

\begin{equation}
P_{ 2} = 1240.000\textnormal{ psia                      }
\end{equation}

\begin{equation}
  h_{ 2,s} = (h_{f} + x_{ 2}h_{fg})_{@P 2} =  577.420 + 0.95\cdot 605.640 = 1152.778
\textnormal{ BTU/lbm                   }
\end{equation}

\begin{equation}
  s_{ 2,s} = (s_{f} + x_{ 2}s_{fg})_{@P 2} =    0.777 + 0.95\cdot   0.587 =    1.335
\textnormal{ BTU/lbm}\cdot\textnormal{R}
\end{equation}

\begin{equation}
h_{ 2,a} = h_{ 2,s}
\end{equation}

\begin{equation}
s_{ 2,a} = s_{ 2,s}
\end{equation}

\begin{equation}
P_{ 3} =  940.000\textnormal{ psia                      }
\end{equation}


HP Turbine:
\begin{equation}
(\dot{m}_{ 1} - \dot{m}_{ 3})h_{ 3,a} = \dot{m}_{ 4}h_{ 4,a} + (\dot{m}_{ 1} - \dot{m}_{ 3} - \dot{m}_{ 4})h_{ 5,a} + \dot{W}_{hpt,a}
\end{equation}

\begin{equation}
\frac{\dot{W}_{hpt,a}}{m_1} = (1 - \frac{\dot{m}_{ 3}}{\dot{m}_{ 1}})h_{ 3,a} - \frac{\dot{m}_{ 4}}{\dot{m}_{ 1}}h_{ 4,a} - (1 - \frac{\dot{m}_{ 3}}{\dot{m}_{ 1}} - \frac{\dot{m}_{ 4}}{\dot{m}_{ 1}})h_{ 5,a}\end{equation}

\begin{equation}
\eta_{hpt} =    0.950 = \frac{\dot{W}_{hpt,a} / \dot{m}_{1}}{\dot{W}_{hpt,s} / \dot{m}_{1}}
\end{equation}


LP Turbine:
\begin{equation}
(\dot{m}_{ 1} - \dot{m}_{ 3} - \dot{m}_{ 4})h_{ 6,a} = \dot{m}_{ 5}h_{ 8,a} + \dot{m}_{ 6}h_{ 9,a} + (\dot{m}_{ 1} - \dot{m}_{ 3} - \dot{m}_{ 4} - \dot{m}_{ 5} - \dot{m}_{ 6})h_{10,a} + \dot{W}_{lpt,a}
\end{equation}

\begin{equation}
\frac{\dot{W}_{lpt,a}}{m_1} = (1 - \frac{\dot{m}_{ 3}}{\dot{m}_{ 1}} - \frac{\dot{m}_{ 4}}{\dot{m}_{ 1}})h_{ 6,a} - \frac{\dot{m}_{ 5}}{\dot{m}_{ 1}}h_{ 8,a} - \frac{\dot{m}_{ 6}}{\dot{m}_{ 1}}h_{ 9,a} - (1 - \frac{\dot{m}_{ 3}}{\dot{m}_{ 1}} - \frac{\dot{m}_{ 4}}{\dot{m}_{ 1}} - \frac{\dot{m}_{ 5}}{\dot{m}_{ 1}} - \frac{\dot{m}_{ 6}}{\dot{m}_{ 1}})h_{10,a}\end{equation}

\begin{equation}
\eta_{lpt} =    0.950 = \frac{\dot{W}_{lpt,a} / \dot{m}_{1}}{\dot{W}_{lpt,s} / \dot{m}_{1}}
\end{equation}


Condensate Pump:
\begin{equation}
(\dot{m}_{ 1} - \dot{m}_{ 3} - \dot{m}_{ 4} - \dot{m}_{ 5} - \dot{m}_{ 6})h_{11,a} = (\dot{m}_{ 1} - \dot{m}_{ 3} - \dot{m}_{ 4} - \dot{m}_{ 5} - \dot{m}_{ 6})h_{12,a} + \dot{W}_{cp ,a}
\end{equation}

\begin{equation}
-\frac{\dot{W}_{cp ,a}}{m_1} = (1 - \frac{\dot{m}_{ 3}}{\dot{m}_{ 1}} - \frac{\dot{m}_{ 4}}{\dot{m}_{ 1}} - \frac{\dot{m}_{ 5}}{\dot{m}_{ 1}} - \frac{\dot{m}_{ 6}}{\dot{m}_{ 1}})h_{12,a} - (1 - \frac{\dot{m}_{ 3}}{\dot{m}_{ 1}} - \frac{\dot{m}_{ 4}}{\dot{m}_{ 1}} - \frac{\dot{m}_{ 5}}{\dot{m}_{ 1}} - \frac{\dot{m}_{ 6}}{\dot{m}_{ 1}})h_{11,a}
\end{equation}


Open Heater:
\begin{equation}
\dot{m}_{ 6}h_{ 9,a} + (\dot{m}_{ 1} - \dot{m}_{ 3} - \dot{m}_{ 4} - \dot{m}_{ 5} - \dot{m}_{ 6})h_{12,a} + (\dot{m}_{ 3} + \dot{m}_{ 4} + \dot{m}_{ 5})h_{15,a} = \dot{m}_{ 1}h_{13,a}
\end{equation}


CB Pump:
\begin{equation}
\dot{m}_{ 1}h_{13,a} = \dot{m}_{ 1}h_{14,a} + \dot{W}_{cbp,a}
\end{equation}

\begin{equation}
-\frac{\dot{W}_{cbp,a}}{m_1} = h_{14,a} - h_{13,a}
\end{equation}


Heat Exchanger 1
\begin{equation}
\dot{m}_{ 4}h_{17,a} + \dot{m}_{ 5}h_{ 8,a} + \dot{m}_{ 3}h_{ 7,a} + \dot{m}_{ 1}h_{14,a} = \dot{m}_{ 1}h_{16,a} + (\dot{m}_{ 3} + \dot{m}_{ 4} + \dot{m}_{ 5})h_{15,a}
\end{equation}


Heat Exchanger 2
\begin{equation}
\dot{m}_{ 1}h_{16,a} + \dot{m}_{ 4}h_{ 4,a} = \dot{m}_{ 1}h_{ 1,a} + \dot{m}_{ 4}h_{17,a}
\end{equation}


FP 1
\begin{equation}
\dot{m}_{ 2}h_{ 1,a} = \dot{m}_{ 2}h_{21,a} + \dot{W}_{fp1,a}
\end{equation}

\begin{equation}
-\frac{\dot{W}_{fp1,a}}{m_1} = \frac{\dot{m}_{ 2}}{\dot{m}_{ 1}}h_{21,a} - \frac{\dot{m}_{ 2}}{\dot{m}_{ 1}}h_{ 1,a}
\end{equation}


FP 2
\begin{equation}
\dot{m}_{ 2}h_{ 1,a} = \dot{m}_{ 2}h_{21,a} + \dot{W}_{fp2,a}
\end{equation}

\begin{equation}
-\frac{\dot{W}_{fp2,a}}{m_1} = \frac{\dot{m}_{ 2}}{\dot{m}_{ 1}}h_{21,a} - \frac{\dot{m}_{ 2}}{\dot{m}_{ 1}}h_{ 1,a}
\end{equation}


\end{document}

